lib/c/lib_intrinsics.h
@@ -30,6 +30,9 @@
   (_addcarry_u64(x1, x2, x3, (long long unsigned int *) x4))
 
 
+#define Lib_IntTypes_Intrinsics_add_carry_u64_void(x1, x2, x3, x4) \
+  (_addcarry_u64(x1, x2, x3, (long long unsigned int *) x4))
+
 /*
    GCC versions prior to 7.2 pass arguments to _subborrow_u{32,64}
    in an incorrect order.
@@ -46,6 +49,10 @@
 
 #define Lib_IntTypes_Intrinsics_sub_borrow_u64(x1, x2, x3, x4)  \
   (_subborrow_u64(x1, x2, x3, (long long unsigned int *) x4))
+
+#define Lib_IntTypes_Intrinsics_sub_borrow_u64_void(x1, x2, x3, x4)  \
+  (_subborrow_u64(x1, x2, x3, (long long unsigned int *) x4))
+
 
 #endif // GCC < 7.2
 
