code/ecdsap256/Hacl.Impl.P256.MontgomeryMultiplication.fst
@@ -31,7 +31,7 @@ val add8_without_carry1: t: widefelem -> t1: widefelem -> result: widefelem  -> 
   (ensures fun h0 _ h1 -> modifies (loc result) h0 h1 /\ wide_as_nat h1 result = wide_as_nat h0 t + wide_as_nat h0 t1)
 
 let add8_without_carry1 t t1 result  = 
-  let _  = add8 t t1 result in 
+  add8_void t t1 result;
     assert_norm (pow2 320 + prime256 * prime256 < pow2 512)
 
 (* inline_for_extraction
