lib/Lib.IntTypes.Intrinsics.fsti
@@ -18,6 +18,16 @@ val add_carry_u64: cin:uint64 -> x:uint64 -> y:uint64 -> r:lbuffer uint64 (size 
        v r + v c * pow2 64 == v x + v y + v cin))
 
 noextract
+val add_carry_u64_void: cin:uint64 -> x:uint64 -> y:uint64 -> r:lbuffer uint64 (size 1) -> 
+  Stack unit 
+    (requires fun h -> live h r /\ v cin <= 1)
+    (ensures  fun h0 _ h1 -> 
+      modifies1 r h0 h1 /\ (
+      let r = Seq.index (as_seq h1 r) 0 in 
+       v r == v x + v y + v cin))
+
+
+noextract
 val sub_borrow_u64: cin:uint64 -> x:uint64 -> y:uint64 -> r:lbuffer uint64 (size 1) -> 
   Stack uint64
     (requires fun h -> live h r /\ v cin <= 1)
@@ -25,3 +35,13 @@ val sub_borrow_u64: cin:uint64 -> x:uint64 -> y:uint64 -> r:lbuffer uint64 (size
       modifies1 r h0 h1 /\ 
       (let r = Seq.index (as_seq h1 r) 0 in 
        v r - v c * pow2 64 == v x - v y - v cin))
+
+
+noextract
+val sub_borrow_u64_void: cin:uint64 -> x:uint64 -> y:uint64 -> r:lbuffer uint64 (size 1) -> 
+  Stack unit
+    (requires fun h -> live h r /\ v cin <= 1)
+    (ensures  fun h0 _ h1 -> 
+      modifies1 r h0 h1 /\ 
+      (let r = Seq.index (as_seq h1 r) 0 in 
+       v r == v x - v y - v cin))
